rocq-brick-libstdcpp/test/g4g/N5_swap_a.v
@@ -12,36 +12,22 @@ Section with_cpp.
   Context `{SPECTRA : !appG APP _Σ}.
 
   #[local] Instance Swap : App.app := mkApp APP.
-  Definition X := requester_C Swap.
-  Hint Resolve X : sl_opacity.
-
   #[program]
-  Definition OS (E : coPset) γ : Ostream :=
-    {| do := Step.requester Swap E γ |}%I.
-  Next Obligation. repeat intro. apply requester_ne; done. Qed.
+    Definition OS γ : Ostream :=
+    AppHandler Swap (⊤ ∖ ↑refinement_rootNS) masks.default γ.
 
-
-  cpp.spec "main()" from source as main_spec with (
-    \prepost{γ osM} _global "std::cout" |-> ostream.R (OS ⊤ γ) osM 1$m
-    \pre AuthSet.frag γ {[ behavior 2 3 ]}
-    \post[Vint 0]  AuthSet.frag γ {[ ""%bs ]}).
-
-  #[program]
-  Definition bs_dos_steps_C (s : bs) (s' : propset (Sts._state (App.lts Swap))) str
-    (ANY_STEPS : AnySteps only_output {[s]} ((fun x => Write x) <$> BS.string_to_bytes str) s') :=
-    \cancelx
-      \using{γ} AuthSet.frag γ {[s]}
-      \proving{K : mpredI} ostream.bs_dos (OS ⊤ γ) str K
-      \through (AuthSet.frag γ s' -∗ K)
-      \end@{mpredI}.
-  Next Obligation.
-    simpl.
-    intros.
-    iIntros "F" (?) "K".
-    rewrite /Step.requester.
-  Admitted.
+  (* NOTE: the following two specializations work around issues with the
+     Spectra packaging which uses bundling. *)
+  Definition gen_X := gen_requester_C Swap.
+  Hint Resolve gen_X : sl_opacity.
+  Definition bs_dos_steps_C := gen_bs_dos_steps_C Swap.(App.lts) Swap.(App.inG).
   Hint Resolve bs_dos_steps_C : sl_opacity.
 
+  cpp.spec "main()" from source as main_spec with (
+    \prepost{γ osM} _global "std::cout" |-> ostream.R (OS γ) osM 1$m
+    \persist Step.updater Swap (⊤ ∖ ↑refinement_rootNS) γ
+    \pre AuthSet.frag γ {[ behavior 2 3 ]}
+    \post[Vint 0]  AuthSet.frag γ {[ ""%bs ]}).
 
   Lemma main_ok : verify[source] "main()".
   Proof.
